\begin{equation}\label{ueqzero}
\begin{bmatrix}
    \dot s \\ \ddot s \\ \dot \phi \\ \ddot \phi
\end{bmatrix} =  \begin{bmatrix}
    0 \\ 0 \\ 0 \\ 0
\end{bmatrix} = \begin{bmatrix}
    \dot{s} \\
    \frac{u}{M}-\frac{F\dot{s}}{M}  \\
    \dot{\phi} \\
     \frac{g\sin\left(\phi \right)}{L}-\frac{u\cos\left(\phi \right)}{LM}+\frac{F\dot{s}\cos\left(\phi \right)}{LM} \\
\end{bmatrix} \rightarrow \mu=0 \rightarrow \underline{x} = \begin{bmatrix}
    s \\ \dot s \\ \phi \\ \dot \phi
\end{bmatrix} = \begin{bmatrix}
    \Re \\
    0 \\
    \pi n, n \in \mathbb{Z} \\
    0 \\
\end{bmatrix}
\end{equation}

